Add Word8Array.copyVec and Word8Array.substring
The first copies part of a string into a byte array,
the second copies part of a byte array into a string.

Proved the spec for copyVec but not yet substring.

characteristic/cfScript.sml
@@ -1306,10 +1306,22 @@ val app_copyaw8aw8_def = Define `
         0 <= do /\ 0 <= so /\ 0 <= l /\
         (Num do + Num l) <= LENGTH wd /\(Num so + Num l) <= LENGTH ws /\
         (H ==>> F * W8ARRAY s ws * W8ARRAY d wd) /\
-        (F * W8ARRAY s ws * 
-             W8ARRAY d (TAKE (Num do) wd ⧺ 
-                        TAKE (Num l) (DROP (Num so) ws) ⧺ 
-                        DROP (Num do + Num l) wd)  
+        (F * W8ARRAY s ws *
+             W8ARRAY d (TAKE (Num do) wd ⧺
+                        TAKE (Num l) (DROP (Num so) ws) ⧺
+                        DROP (Num do + Num l) wd)
+            ==>> Q (Val (Conv NONE [])))) /\
+     Q ==e> POST_F)`
+
+val app_copystraw8_def = Define `
+  app_copystraw8 s so l d do H Q =
+    ((?wd F.
+        0 <= do /\ 0 <= so /\ 0 <= l /\
+        (Num do + Num l) <= LENGTH wd /\(Num so + Num l) <= LENGTH s /\
+        (H ==>> F * W8ARRAY d wd) /\
+        (F * W8ARRAY d (TAKE (Num do) wd ⧺
+                        MAP (n2w o ORD) (TAKE (Num l) (DROP (Num so) s)) ⧺
+                        DROP (Num do + Num l) wd)
             ==>> Q (Val (Conv NONE [])))) /\
      Q ==e> POST_F)`
 
@@ -1534,6 +1546,16 @@ val cf_copyaw8aw8_def = Define `
       exp2v env xdo = SOME (Litv (IntLit do)) /\
       app_copyaw8aw8 s so l d do H Q)`
 
+val cf_copystraw8_def = Define `
+  cf_copystraw8 xs xso xl xd xdo = \env. local (\H Q.
+    ?s so l d do.
+      exp2v env xs = SOME (Litv (StrLit s)) /\
+      exp2v env xd = SOME d /\
+      exp2v env xl = SOME (Litv (IntLit l)) /\
+      exp2v env xso = SOME (Litv (IntLit so)) /\
+      exp2v env xdo = SOME (Litv (IntLit do)) /\
+      app_copystraw8 s so l d do H Q)`
+
 val cf_wordFromInt_W8_def = Define `
   cf_wordFromInt_W8 xi = \env. local (\H Q.
     ?i.
@@ -1699,6 +1721,10 @@ val cf_def = tDefine "cf" `
           (case args of
              | [s; so; l; d; do] => cf_copyaw8aw8 s so l d do
              | _ => cf_bottom)
+        | CopyStrAw8 =>
+          (case args of
+             | [s; so; l; d; do] => cf_copystraw8 s so l d do
+             | _ => cf_bottom)
         | WordFromInt W8 =>
           (case args of
              | [i] => cf_wordFromInt_W8 i
@@ -1777,6 +1803,7 @@ val cf_defs = [
   cf_aw8length_def,
   cf_aw8update_def,
   cf_copyaw8aw8_def,
+  cf_copystraw8_def,
   cf_wordFromInt_W8_def,
   cf_wordFromInt_W64_def,
   cf_wordToInt_W8_def,
@@ -2644,6 +2671,38 @@ val cf_sound = Q.store_thm ("cf_sound",
       progress SPLIT3_of_SPLIT_emp3 \\ instantiate
     ) \\
     try_finally (
+      (* CopyStrAw8 *)
+      Q.REFINE_EXISTS_TAC `Val v'` \\ simp [] \\ cf_evaluate_step_tac \\
+      GEN_EXISTS_TAC "ck" `st.clock` \\ fs [with_clock_self] \\
+      cf_exp2v_evaluate_tac `st` \\
+      fs [st2heap_def,app_copystraw8_def] \\
+      fs [W8ARRAY_def] \\
+      fs [SEP_EXISTS, cond_def, SEP_IMP_def, STAR_def, one_def, cell_def] \\
+      first_x_assum progress
+      \\ rename1 `d = Loc ld` \\ rw [] \\
+      assume_tac (GEN_ALL Mem_NOT_IN_ffi2heap) \\
+      (rename1 `W8array _` \\
+        `Mem ld (W8array wd) IN (store2heap st.refs)` by SPLIT_TAC) \\
+      progress store2heap_IN_LENGTH \\ progress store2heap_IN_EL \\
+      fs [do_app_def, store_lookup_def, store_assign_def, store_v_same_type_def, IMPLODE_EXPLODE_I] \\
+      fs[copy_array_def,integerTheory.INT_ABS] \\
+      rpt(full_case_tac THEN1 (irule FALSITY \\ intLib.ARITH_TAC)) \\
+      IF_CASES_TAC \\ fs[] \\ TRY (`F` by intLib.ARITH_TAC) \\
+      IF_CASES_TAC \\ fs[ws_to_chars_def,chars_to_ws_def] \\ TRY (`F` by intLib.ARITH_TAC) \\
+      fs [evaluateTheory.list_result_def] \\
+      qmatch_goalsub_abbrev_tac`W8array wd'` \\
+      qexists_tac `Mem ld (W8array wd') INSERT u` \\
+      qexists_tac `{}` \\ mp_tac store2heap_IN_unique_key \\ rpt strip_tac
+      THEN1 (progress_then (fs o sing) store2heap_LUPDATE \\ SPLIT_TAC) \\
+      first_assum irule \\
+      qexists_tac`u` \\
+      qexists_tac`{Mem ld (W8array wd')}` \\ fs[Abbr`wd'`] \\
+      `Num do + Num l = Num (do +l)` by intLib.ARITH_TAC \\
+      simp[MAP_TAKE,MAP_DROP,MAP_MAP_o,o_DEF,integer_wordTheory.i2w_pos] \\
+      simp[GSYM o_DEF,n2w_ORD_CHR_w2n] \\
+      SPLIT_TAC
+    ) \\
+    try_finally (
       (* CopyAw8Aw8 *)
       Q.REFINE_EXISTS_TAC `Val v'` \\ simp [] \\ cf_evaluate_step_tac \\
       GEN_EXISTS_TAC "ck" `st.clock` \\ fs [with_clock_self] \\
@@ -2651,7 +2710,7 @@ val cf_sound = Q.store_thm ("cf_sound",
       fs [st2heap_def,app_copyaw8aw8_def] \\
       fs [W8ARRAY_def] \\
       fs [SEP_EXISTS, cond_def, SEP_IMP_def, STAR_def, one_def, cell_def] \\
-      first_x_assum progress 
+      first_x_assum progress
       \\ rename1 `s = Loc ls` \\ rename1 `d = Loc ld` \\ rw [] \\
       assume_tac (GEN_ALL Mem_NOT_IN_ffi2heap) \\
       (rename1 `W8array _` \\
